cklr/InjectFootprint.v
@@ -2706,4 +2706,3 @@ Proof.
         intros [E F]. split; eauto.
     + repeat rstep; eauto.
 Qed.
-
